steel/Zeta.Steel.ThreadLogMap.fst
@@ -1,0 +1,91 @@
+module Zeta.Steel.ThreadLogMap
+open FStar.Ghost
+open FStar.Seq
+open Zeta.Steel.FormatsManual
+open Zeta.Steel.ApplicationTypes
+open Zeta.Steel.ApplicationTypes
+open Steel.ST.Util
+module FAP = Zeta.Steel.FractionalAnchoredPreorder
+module PM = Zeta.Steel.PCMMap
+module M = Zeta.Steel.ThreadStateModel
+
+let log = Seq.seq log_entry_base
+
+let log_grows :Preorder.preorder log
+  = let open FStar.Seq in
+    fun (s1 s2:log) ->
+      length s1 <= length s2 /\
+      (forall (i:nat).{:pattern (Seq.index s1 i) \/ (Seq.index s2 i)}
+         i < length s1 ==> index s1 i == index s2 i)
+
+let committed_log_entries_split (l0 l1 l2: log)
+  : Lemma
+    (requires
+      M.committed_log_entries l0 == M.committed_log_entries l2 /\
+      log_grows l0 l1 /\
+      log_grows l1 l2)
+    (ensures
+            M.committed_log_entries l0 == M.committed_log_entries l1)
+  = admit()
+
+
+let anchor : log -> log -> prop
+  = fun l0 l1 ->
+      log_grows l0 l1 /\
+      M.committed_log_entries l0 == M.committed_log_entries l1
+
+let anchor_refl : squash (forall l. anchor l l) = ()
+let anchor_pre : squash (forall l0 l1. anchor l0 l1 ==> log_grows l0 l1) = ()
+let anchor_split : squash (forall x z. x `anchor` z  ==> (forall y. log_grows x y /\ log_grows y z ==> x `anchor` y)) =
+  introduce forall x. _
+  with introduce forall z. x `anchor` z  ==> (forall y. log_grows x y /\ log_grows y z ==> x `anchor` y)
+  with introduce _ ==> _
+  with _. introduce forall y. _
+  with introduce _ ==> _
+  with _. committed_log_entries_split x y z
+let anchors : FAP.anchor_rel log_grows = anchor
+
+let fap = FAP.pcm #log #log_grows #anchors
+let pcm = PM.pointwise tid fap
+let aval = FAP.knowledge anchors
+let has_key  (m:PM.map tid aval) (tid:tid) = FAP.Owns? (Map.sel m tid)
+let owns_key (m:PM.map tid aval) (tid:tid) =
+  has_key m tid /\
+  FAP.avalue_owns (FAP.Owns?._0 (Map.sel m tid))
+let avalue_of (m:PM.map tid aval) (tid:tid { has_key m tid }) =
+  (FAP.Owns?._0 (Map.sel m tid))
+let get (m:PM.map tid aval) (tid:tid { has_key m tid }) =
+  Steel.Preorder.curval (FAP.avalue_val (avalue_of m tid))
+let put (m:PM.map tid aval) (tid:tid { has_key m tid }) (l:log {get m tid `log_grows` l}) =
+  Map.upd m tid (FAP.Owns (FAP.avalue_update_value (FAP.Owns?._0 (Map.sel m tid)) l))
+
+let update_value (l:log)
+                 (m:PM.map tid aval)
+                 (tid:tid {
+                   owns_key m tid /\ //if you have full ownership of key
+                   get m tid `log_grows` l //you can update it wrt the preorder only
+                 })
+  : PCM.frame_preserving_upd pcm m (put m tid l)
+  = PM.lift_fp_upd _ _ (FAP.update_value (FAP.Owns?._0 (Map.sel m tid)) l) m tid
+
+let owns_anchored_key (m:PM.map tid aval) (tid:tid) =
+  has_key m tid /\
+  FAP.avalue_owns_anchored (FAP.Owns?._0 (Map.sel m tid))
+
+let put_anchored (m:PM.map tid aval)
+                 (tid:tid { has_key m tid })
+                 (l:log {
+                   get m tid `log_grows` l /\
+                   l `FAP.compat_with_any_anchor_of` (avalue_of m tid)
+                 }) =
+  Map.upd m tid (FAP.Owns (FAP.avalue_update_anchored_value (FAP.Owns?._0 (Map.sel m tid)) l))
+
+let update_anchored_value (l:log)
+                          (m:PM.map tid aval)
+                          (tid:tid {
+                            owns_anchored_key m tid /\ //if you own an anchored key, you can update if you respect
+                            get m tid `log_grows` l /\ //the preorder
+                            l `FAP.compat_with_any_anchor_of` (avalue_of m tid) //and respect any anchor of the current value
+                          })
+  : PCM.frame_preserving_upd pcm m (put_anchored m tid l)
+  = PM.lift_fp_upd _ _ (FAP.update_anchored_value (FAP.Owns?._0 (Map.sel m tid)) l) m tid
